annotated/append_verif.v
@@ -29,9 +29,11 @@ Proof.
 start_function f_append_hint.
 forwardD.
 * forwardD.
-  rewrite listrep_null. normalize.
-  Exists y.
-  simpl; entailer!.
+  {
+    rewrite listrep_null. normalize.
+    Exists y.
+    simpl; entailer!.
+  }
 * forwardD.
   forwardD.
   {
@@ -90,60 +92,9 @@ forwardD.
     }
     (* else branch *)
     forwardD.
-    forwardD.
-  (* lazymatch goal with
-  (* entailment *)
-  | |- let d := @abbreviate _ _ in ENTAIL _, _ |-- ?Post =>
-      intro d; clear d;
-      is_evar Post;
-        repeat first
-        [ apply delta_derives_refl; fail 2
-        | match reverse goal with
-          | H : Intro_tag ?x |- _ =>
-            Exists x; clear H; idtac x
-          end
-        ]end. *)
-    (* 
-    Lemma revert_evar : forall {A} (x : A) P (Q : assert),
-      EX x, P x |-- Q -> P x |-- Q.
-    Proof.
-      intros. eapply derives_trans. 2 : apply H. EExists. apply derives_refl.
-    Qed.
-    Lemma delta_remove : forall Delta P Q,
-      P |-- Q -> ENTAIL Delta, P |-- Q.
-    Proof.
-      intros. apply andp_left2. assumption.
-    Qed.
-    apply delta_remove.
-    match goal with
-    | |- ?P |-- ?Q =>
-      match P with
-      | ?P' u => idtac P'
-      end
-    end.
-    eapply (revert_evar u).
-    eapply exp_right with t.
-    Exists u. Exists u. simpl in Post. Exists t. Exists s1b. Exists a. apply delta_derives_refl. *)
-    (* match goal with
-          | H : Intros_tag ?x |- _ =>
-            idtac x; Exists x
-          end.
-          match goal with
-          | H : Intros_tag ?x |- _ =>
-            idtac x; Exists x
-          end.
-          Exists t.
-          match goal with
-          | H : Intros_tag ?x |- _ =>
-            idtac x; Exists x
-          end.
-    {
-      Exists u. Exists t.
-      Exists a. Exists s1b. Exists t. u H13. apply delta_derives_refl.
-      (*  entailer!. rewrite (proj1 H4 (eq_refl _)). simpl. cancel. *)
-    } *)
   }
-  { forwardD.
+  { (* intro d. simpl annotation_proofauto.rev. Intros xx. Intros xx0. Intros xx1. Intros xx2. revert d. *)
+    forwardD.
     forwardD.
     forwardD.
     forwardD.
@@ -153,8 +104,9 @@ forwardD.
       Exists x.
       entailer!.
       rewrite (proj1 H9 (eq_refl _)). simpl.
-      unfold listrep at 3; fold listrep. normalize.
-      pull_right (listrep sh (a :: s2) t -* listrep sh ((a0 :: s1b0) ++ s2) x).
+      unfold listrep at 3; fold listrep.
+      normalize.
+      pull_right (listrep sh (a0 :: s2) t -* listrep sh ((a :: s1b) ++ s2) x).
       apply modus_ponens_wand'.
       unfold listrep at 2; fold listrep. Exists y; auto.
     }
